Tidying the Okasaki data structures examples.

examples/miniML/hol2miniml/okasaki-examples/LeftistHeapScript.sml
@@ -1,90 +1,90 @@
-open bossLib Theory Parse boolTheory pairTheory Defn Tactic boolLib bagTheory
-open relationTheory bagLib miscTheory lcsymtacs;
+open preamble
+open bagTheory bagLib miscTheory;
 open ml_translatorLib;
 
 val fs = full_simp_tac (srw_ss ())
 val rw = srw_tac []
-val wf_rel_tac = WF_REL_TAC
-val induct_on = Induct_on
-val cases_on = Cases_on;
-val every_case_tac = BasicProvers.EVERY_CASE_TAC;
-val full_case_tac = BasicProvers.FULL_CASE_TAC;
 
 val _ = new_theory "LeftistHeap"
 
+(* Okasaki page 20 *)
+
 val _ = Hol_datatype `
-heap = Empty | Node of num => 'a => heap => heap`;
+heap = Empty | Tree of num => 'a => heap => heap`;
 
-val leftist_heap_to_bag_def = Define `
-(leftist_heap_to_bag Empty = {||}) ∧
-(leftist_heap_to_bag (Node _ x h1 h2) =
-  BAG_INSERT x (BAG_UNION (leftist_heap_to_bag h1) (leftist_heap_to_bag h2)))`;
+val heap_to_bag_def = Define `
+(heap_to_bag Empty = {||}) ∧
+(heap_to_bag (Tree _ x h1 h2) =
+  BAG_INSERT x (BAG_UNION (heap_to_bag h1) (heap_to_bag h2)))`;
 
-val rank_def = Define `
+val rank_def = mlDefine `
 (rank Empty = 0) ∧
-(rank (Node r _ _ _) = r)`;
+(rank (Tree r _ _ _) = r)`;
 
-val leftist_heap_ok_def = Define `
-(leftist_heap_ok get_key leq Empty = T) ∧
-(leftist_heap_ok get_key leq (Node _ x h1 h2) =
-  leftist_heap_ok get_key leq h1 ∧
-  leftist_heap_ok get_key leq h2 ∧
-  BAG_EVERY (\y. leq (get_key x) (get_key y)) (leftist_heap_to_bag h1) ∧
-  BAG_EVERY (\y. leq (get_key x) (get_key y)) (leftist_heap_to_bag h2) ∧
+val is_heap_ordered_def = Define `
+(is_heap_ordered get_key leq Empty = T) ∧
+(is_heap_ordered get_key leq (Tree _ x h1 h2) =
+  is_heap_ordered get_key leq h1 ∧
+  is_heap_ordered get_key leq h2 ∧
+  BAG_EVERY (\y. leq (get_key x) (get_key y)) (heap_to_bag h1) ∧
+  BAG_EVERY (\y. leq (get_key x) (get_key y)) (heap_to_bag h2) ∧
   rank h1 ≥ rank h2)`;
 
-val make_node_def = Define `
+val make_node_def = mlDefine `
 make_node x a b =
   if rank a >= rank b then
-    Node (rank b + 1) x a b
+    Tree (rank b + 1) x a b
   else
-    Node (rank a + 1) x b a`;
+    Tree (rank a + 1) x b a`;
 
-val _ = Define `
+val _ = mlDefine `
 empty = Empty`;
 
-val is_empty_def = Define `
+val is_empty_def = mlDefine `
 (is_empty Empty = T) ∧
 (is_empty _ = F)`;
 
-val merge_def = Define `
+val merge_def = mlDefine `
 (merge get_key leq h Empty = h) ∧
 (merge get_key leq Empty h = h) ∧
-(merge get_key leq (Node n1 x a1 b1) (Node n2 y a2 b2) =
+(merge get_key leq (Tree n1 x a1 b1) (Tree n2 y a2 b2) =
   if leq (get_key x) (get_key y) then
-    make_node x a1 (merge get_key leq b1 (Node n2 y a2 b2))
+    make_node x a1 (merge get_key leq b1 (Tree n2 y a2 b2))
   else
-    make_node y a2 (merge get_key leq (Node n1 x a1 b1) b2))`;
+    make_node y a2 (merge get_key leq (Tree n1 x a1 b1) b2))`;
 
 val merge_ind = fetch "-" "merge_ind"
 
-val insert_def = Define `
-insert get_key leq x h = merge get_key leq (Node 1 x Empty Empty) h`;
+val insert_def = mlDefine `
+insert get_key leq x h = merge get_key leq (Tree 1 x Empty Empty) h`;
 
-val find_min_def = Define `
-find_min (Node _ x _ _) = x`;
+val find_min_def = mlDefine `
+find_min (Tree _ x _ _) = x`;
 
-val delete_min_def = Define `
-delete_min get_key leq (Node _ x a b) = merge get_key leq a b`;
+val delete_min_def = mlDefine `
+delete_min get_key leq (Tree _ x a b) = merge get_key leq a b`;
 
-val leftist_heap_merge_bag = Q.store_thm ("leftist_heap_merge_bag",
+
+(* Functional correctness proof *)
+
+val merge_bag = Q.store_thm ("merge_bag",
 `!get_key leq h1 h2.
-  leftist_heap_to_bag (merge get_key leq h1 h2) =
-  BAG_UNION (leftist_heap_to_bag h1) (leftist_heap_to_bag h2)`,
+  heap_to_bag (merge get_key leq h1 h2) =
+  BAG_UNION (heap_to_bag h1) (heap_to_bag h2)`,
 HO_MATCH_MP_TAC merge_ind >>
 srw_tac [BAG_ss]
-        [merge_def, leftist_heap_to_bag_def, make_node_def, BAG_INSERT_UNION]);
+        [merge_def, heap_to_bag_def, make_node_def, BAG_INSERT_UNION]);
 
-val leftist_heap_merge_ok = Q.store_thm ("leftist_heap_merge_ok",
+val merge_heap_ordered = Q.store_thm ("merge_heap_ordered",
 `!get_key leq h1 h2.
   WeakLinearOrder leq ∧
-  leftist_heap_ok get_key leq h1 ∧
-  leftist_heap_ok get_key leq h2
+  is_heap_ordered get_key leq h1 ∧
+  is_heap_ordered get_key leq h2
   ⇒
-  leftist_heap_ok get_key leq (merge get_key leq h1 h2)`,
+  is_heap_ordered get_key leq (merge get_key leq h1 h2)`,
 HO_MATCH_MP_TAC merge_ind >>
-rw [merge_def, leftist_heap_ok_def, make_node_def, leftist_heap_merge_bag] >>
-rw [leftist_heap_to_bag_def] >>
+rw [merge_def, is_heap_ordered_def, make_node_def, merge_bag] >>
+rw [heap_to_bag_def] >>
 fs [BAG_EVERY] >|
 [metis_tac [WeakLinearOrder, WeakOrder, transitive_def],
  metis_tac [WeakLinearOrder, WeakOrder, transitive_def],
@@ -99,59 +99,45 @@ fs [BAG_EVERY] >|
  metis_tac [WeakLinearOrder, WeakOrder, transitive_def, WeakLinearOrder_neg],
  decide_tac]);
 
-val leftist_heap_insert_bag = Q.store_thm ("leftist_heap_insert_bag",
+val insert_bag = Q.store_thm ("insert_bag",
 `!h get_key leq x.
-  leftist_heap_to_bag (insert get_key leq x h) =
-  BAG_INSERT x (leftist_heap_to_bag h)`,
-rw [insert_def, leftist_heap_merge_bag, leftist_heap_to_bag_def,
+  heap_to_bag (insert get_key leq x h) = BAG_INSERT x (heap_to_bag h)`,
+rw [insert_def, merge_bag, heap_to_bag_def,
     BAG_INSERT_UNION]);
 
-val leftist_heap_insert_ok = Q.store_thm ("leftist_heap_insert_ok",
+val insert_heap_ordered = Q.store_thm ("insert_heap_ordered",
 `!get_key leq x h.
-  WeakLinearOrder leq ∧ leftist_heap_ok get_key leq h
+  WeakLinearOrder leq ∧ is_heap_ordered get_key leq h
   ⇒
-  leftist_heap_ok get_key leq (insert get_key leq x h)`,
+  is_heap_ordered get_key leq (insert get_key leq x h)`,
 rw [insert_def] >>
-`leftist_heap_ok get_key leq (Node 1 x Empty Empty)`
-         by rw [leftist_heap_ok_def, leftist_heap_to_bag_def] >>
-metis_tac [leftist_heap_merge_ok]);
+`is_heap_ordered get_key leq (Tree 1 x Empty Empty)`
+         by rw [is_heap_ordered_def, heap_to_bag_def] >>
+metis_tac [merge_heap_ordered]);
 
-val leftist_heap_find_min_thm = Q.store_thm ("leftist_heap_find_min_thm",
+val find_min_correct = Q.store_thm ("find_min_correct",
 `!h get_key leq.
-  WeakLinearOrder leq ∧ (h ≠ Empty) ∧ leftist_heap_ok get_key leq h
+  WeakLinearOrder leq ∧ (h ≠ Empty) ∧ is_heap_ordered get_key leq h
   ⇒
-  BAG_IN (find_min h) (leftist_heap_to_bag h) ∧
-  (!y. BAG_IN y (leftist_heap_to_bag h) ⇒
-       leq (get_key (find_min h)) (get_key y))`,
+  BAG_IN (find_min h) (heap_to_bag h) ∧
+  (!y. BAG_IN y (heap_to_bag h) ⇒ leq (get_key (find_min h)) (get_key y))`,
 rw [] >>
 cases_on `h` >>
-fs [find_min_def, leftist_heap_to_bag_def, leftist_heap_ok_def] >>
+fs [find_min_def, heap_to_bag_def, is_heap_ordered_def] >>
 fs [BAG_EVERY] >>
 metis_tac [WeakLinearOrder, WeakOrder, reflexive_def]);
 
-val leftist_heap_delete_min_thm = Q.store_thm ("leftist_heap_delete_min_thm",
+val delete_min_correct = Q.store_thm ("delete_min_correct",
 `!h get_key leq.
-  WeakLinearOrder leq ∧
-  (h ≠ Empty) ∧
-  leftist_heap_ok get_key leq h
+  WeakLinearOrder leq ∧ (h ≠ Empty) ∧ is_heap_ordered get_key leq h
   ⇒
-  leftist_heap_ok get_key leq (delete_min get_key leq h) ∧
-  (leftist_heap_to_bag (delete_min get_key leq h) =
-   BAG_DIFF (leftist_heap_to_bag h) (EL_BAG (find_min h)))`,
+  is_heap_ordered get_key leq (delete_min get_key leq h) ∧
+  (heap_to_bag (delete_min get_key leq h) =
+   BAG_DIFF (heap_to_bag h) (EL_BAG (find_min h)))`,
 rw [] >>
 cases_on `h` >>
-fs [delete_min_def, leftist_heap_ok_def, leftist_heap_merge_bag] >-
-metis_tac [leftist_heap_merge_ok] >>
-rw [leftist_heap_to_bag_def, find_min_def, BAG_DIFF_INSERT2]);
-
-
-val res = translate is_empty_def;
-val res = translate rank_def;
-val res = translate make_node_def;
-val res = translate listTheory.APPEND;
-val res = translate merge_def;
-val res = translate insert_def;
-val res = translate find_min_def;
-val res = translate delete_min_def;
+fs [delete_min_def, is_heap_ordered_def, merge_bag] >-
+metis_tac [merge_heap_ordered] >>
+rw [heap_to_bag_def, find_min_def, BAG_DIFF_INSERT2]);
 
 val _ = export_theory ();
