examples/miniML/hol2miniml/okasaki-examples/SplayHeapScript.sml
@@ -1,62 +1,59 @@
-open bossLib Theory Parse boolTheory pairTheory Defn Tactic boolLib bagTheory
-open relationTheory bagLib miscTheory lcsymtacs ml_translatorLib;
+open preamble
+open bagTheory relationTheory bagLib miscTheory ml_translatorLib;
 
-val fs = full_simp_tac (srw_ss ())
 val rw = srw_tac []
-val wf_rel_tac = WF_REL_TAC
-val induct_on = Induct_on
-val cases_on = Cases_on;
-val every_case_tac = BasicProvers.EVERY_CASE_TAC;
-val full_case_tac = BasicProvers.FULL_CASE_TAC;
+val fs = full_simp_tac (srw_ss())
 
 val _ = new_theory "SplayHeap"
 
+(* Okasaki page 50 *)
+
 val _ = Hol_datatype `
-heap = Empty | Node of heap => 'a => heap`;
+heap = Empty | Tree of heap => 'a => heap`;
 
-val splay_heap_to_bag_def = Define `
-(splay_heap_to_bag Empty = {||}) ∧
-(splay_heap_to_bag (Node h1 x h2) =
-  BAG_INSERT x (BAG_UNION (splay_heap_to_bag h1) (splay_heap_to_bag h2)))`;
+val heap_to_bag_def = Define `
+(heap_to_bag Empty = {||}) ∧
+(heap_to_bag (Tree h1 x h2) =
+  BAG_INSERT x (BAG_UNION (heap_to_bag h1) (heap_to_bag h2)))`;
 
-val splay_heap_ok_def = Define `
-(splay_heap_ok get_key leq Empty = T) ∧
-(splay_heap_ok get_key leq (Node h1 x h2) =
-  splay_heap_ok get_key leq h1 ∧
-  splay_heap_ok get_key leq h2 ∧
-  BAG_EVERY (\y. leq (get_key y) (get_key x)) (splay_heap_to_bag h1) ∧
-  BAG_EVERY (\y. leq (get_key x) (get_key y)) (splay_heap_to_bag h2))`;
+val is_heap_ordered_def = Define `
+(is_heap_ordered get_key leq Empty = T) ∧
+(is_heap_ordered get_key leq (Tree h1 x h2) =
+  is_heap_ordered get_key leq h1 ∧
+  is_heap_ordered get_key leq h2 ∧
+  BAG_EVERY (\y. leq (get_key y) (get_key x)) (heap_to_bag h1) ∧
+  BAG_EVERY (\y. leq (get_key x) (get_key y)) (heap_to_bag h2))`;
 
-val _ = Define `
+val _ = mlDefine `
 empty = Empty`;
 
-val is_empty_def = Define `
+val is_empty_def = mlDefine `
 (is_empty Empty = T) ∧
 (is_empty _ = F)`;
 
-val partition_def = Define `
+val partition_def = mlDefine `
 (partition get_key leq pivot Empty = (Empty, Empty)) ∧
-(partition get_key leq pivot (Node a x b) =
+(partition get_key leq pivot (Tree a x b) =
   if leq (get_key x) (get_key pivot) then
     (case b of
-        Empty => (Node a x b, Empty)
-      | Node b1 y b2 =>
+        Empty => (Tree a x b, Empty)
+      | Tree b1 y b2 =>
           if leq (get_key y) (get_key pivot) then
             let (small, big) = partition get_key leq pivot b2 in
-              (Node (Node a x b1) y small, big)
+              (Tree (Tree a x b1) y small, big)
           else
             let (small, big) = partition get_key leq pivot b1 in
-              (Node a x small, Node big y b2))
+              (Tree a x small, Tree big y b2))
   else
     (case a of
-        Empty => (Empty, Node a x b)
-      | Node a1 y a2 =>
+        Empty => (Empty, Tree a x b)
+      | Tree a1 y a2 =>
           if leq (get_key y) (get_key pivot) then
             let (small, big) = partition get_key leq pivot a2 in
-              (Node a1 y small, Node big x b)
+              (Tree a1 y small, Tree big x b)
           else
             let (small, big) = partition get_key leq pivot a1 in
-              (small, Node big y (Node a2 x b))))`;
+              (small, Tree big y (Tree a2 x b))))`;
 
 val partition_ind = fetch "-" "partition_ind"
 val heap_size_def = fetch "-" "heap_size_def"
@@ -65,8 +62,7 @@ val partition_size = Q.prove (
 `!get_key leq p h1 h2 h3.
   ((h2,h3) = partition get_key leq p h1)
   ⇒
-  heap_size f h2 ≤ heap_size f h1 ∧
-  heap_size f h3 ≤ heap_size f h1`,
+  heap_size f h2 ≤ heap_size f h1 ∧ heap_size f h3 ≤ heap_size f h1`,
 recInduct partition_ind >>
 rw [heap_size_def, partition_def] >>
 every_case_tac >>
@@ -78,21 +74,57 @@ fs [LET_THM] >>
 rw [heap_size_def] >>
 decide_tac);
 
+val insert_def = mlDefine `
+insert get_key leq x t =
+  let (a, b) = partition get_key leq x t in
+    Tree a x b`;
+
+val merge_def = tDefine "merge" `
+(merge get_key leq Empty h2 = h2) ∧
+(merge get_key leq (Tree a x b) h2 =
+  let (ta, tb) = partition get_key leq x h2 in
+    Tree (merge get_key leq ta a) x (merge get_key leq tb b))`
+(WF_REL_TAC `measure (\(_,x,y,z).  heap_size (\_.1) y + heap_size (\_.1) z)` >>
+ rw [] >>
+ imp_res_tac partition_size >>
+ pop_assum (MP_TAC o Q.SPEC `(λ_.1)`) >>
+ pop_assum (MP_TAC o Q.SPEC `(λ_.1)`) >>
+ full_simp_tac (srw_ss() ++ ARITH_ss) [partition_size]);
+
+val _ = translate merge_def
+
+val merge_ind = fetch "-" "merge_ind"
+
+val find_min_def = mlDefine `
+(find_min (Tree Empty x b) = x) ∧
+(find_min (Tree a x b) = find_min a)`;
+
+val find_min_ind = fetch "-" "find_min_ind"
+
+val delete_min_def = mlDefine `
+(delete_min (Tree Empty x b) = b) ∧
+(delete_min (Tree (Tree Empty x b) y c) = Tree b y c) ∧
+(delete_min (Tree (Tree a x b) y c) = Tree (delete_min a) x (Tree b y c))`;
+
+val delete_min_ind = fetch "-" "delete_min_ind"
+
+
+(* Functional correctnes proof *)
+
 val partition_bags = Q.prove (
 `!get_key leq p h1 h2 h3.
   ((h2,h3) = partition get_key leq p h1)
   ⇒
-  (splay_heap_to_bag h1 =
-   BAG_UNION (splay_heap_to_bag h2) (splay_heap_to_bag h3))`,
+  (heap_to_bag h1 = BAG_UNION (heap_to_bag h2) (heap_to_bag h3))`,
 recInduct partition_ind >>
-rw [partition_def, splay_heap_to_bag_def] >>
+rw [partition_def, heap_to_bag_def] >>
 every_case_tac >>
 fs [] >>
-rw [splay_heap_to_bag_def] >>
+rw [heap_to_bag_def] >>
 cases_on `partition get_key leq pivot h0` >>
 cases_on `partition get_key leq pivot h` >>
 fs [LET_THM] >>
-rw [splay_heap_to_bag_def, BAG_UNION_INSERT] >>
+rw [heap_to_bag_def, BAG_UNION_INSERT] >>
 metis_tac [ASSOC_BAG_UNION, COMM_BAG_UNION, BAG_INSERT_commutes]);
 
 val partition_split = Q.prove (
@@ -100,179 +132,145 @@ val partition_split = Q.prove (
   transitive leq ∧
   trichotomous leq ∧
   ((h2,h3) = partition get_key leq p h1) ∧
-  splay_heap_ok get_key leq h1
+  is_heap_ordered get_key leq h1
   ⇒
-  BAG_EVERY (\y. leq (get_key y) (get_key p)) (splay_heap_to_bag h2) ∧
-  BAG_EVERY (\y. ¬leq (get_key y) (get_key p)) (splay_heap_to_bag h3)`,
+  BAG_EVERY (\y. leq (get_key y) (get_key p)) (heap_to_bag h2) ∧
+  BAG_EVERY (\y. ¬leq (get_key y) (get_key p)) (heap_to_bag h3)`,
 recInduct partition_ind >>
-rw [partition_def, splay_heap_to_bag_def, splay_heap_ok_def] >>
+rw [partition_def, heap_to_bag_def, is_heap_ordered_def] >>
 every_case_tac >>
 fs [] >>
 rw [] >>
-fs [splay_heap_ok_def, splay_heap_to_bag_def] >>
+fs [is_heap_ordered_def, heap_to_bag_def] >>
 cases_on `partition get_key leq pivot h0` >>
 cases_on `partition get_key leq pivot h` >>
-fs [LET_THM, splay_heap_to_bag_def] >>
+fs [LET_THM, heap_to_bag_def] >>
 rw [] >>
 fs [BAG_EVERY, transitive_def, trichotomous] >>
 metis_tac []);
 
-val partition_ok_lem = Q.prove (
+val partition_heap_ordered_lem = Q.prove (
 `!get_key leq p h1 h2 h3.
   (partition get_key leq p h1 = (h2, h3)) ⇒
-  BAG_EVERY P (splay_heap_to_bag h1) ⇒
-  BAG_EVERY P (splay_heap_to_bag h2) ∧
-  BAG_EVERY P (splay_heap_to_bag h3)`,
+  BAG_EVERY P (heap_to_bag h1) ⇒
+  BAG_EVERY P (heap_to_bag h2) ∧ BAG_EVERY P (heap_to_bag h3)`,
 rw [] >>
-`splay_heap_to_bag h1 =
- BAG_UNION (splay_heap_to_bag h2) (splay_heap_to_bag h3)`
+`heap_to_bag h1 =
+ BAG_UNION (heap_to_bag h2) (heap_to_bag h3)`
           by metis_tac [partition_bags] >>
 rw [] >>
-fs [] >>
+fs [BAG_EVERY_UNION] >>
 rw []);
 
-val partition_ok = Q.prove (
+val partition_heap_ordered = Q.prove (
 `!get_key leq p h1 h2 h3.
   WeakLinearOrder leq ∧
   ((h2,h3) = partition get_key leq p h1) ∧
-  splay_heap_ok get_key leq h1
+  is_heap_ordered get_key leq h1
   ⇒
-  splay_heap_ok get_key leq h2 ∧
-  splay_heap_ok get_key leq h3`,
+  is_heap_ordered get_key leq h2 ∧ is_heap_ordered get_key leq h3`,
 recInduct partition_ind >>
-RW_TAC pure_ss [] >>
+RW_TAC pure_ss [] >-
+fs [partition_def, is_heap_ordered_def] >-
+fs [partition_def, is_heap_ordered_def] >>
 cases_on `leq (get_key x) (get_key pivot)` >>
-fs [partition_def, splay_heap_ok_def] >>
+fs [partition_def, is_heap_ordered_def] >>
 every_case_tac >>
 fs [] >>
 rw [] >>
 cases_on `partition get_key leq pivot h0` >>
 cases_on `partition get_key leq pivot h` >>
-fs [LET_THM, splay_heap_ok_def, splay_heap_to_bag_def] >>
+fs [LET_THM, is_heap_ordered_def, heap_to_bag_def] >>
 rw [] >-
 (fs [BAG_EVERY] >>
  metis_tac [transitive_def, WeakLinearOrder, WeakOrder]) >-
-metis_tac [partition_ok_lem] >-
-metis_tac [partition_ok_lem] >-
-metis_tac [partition_ok_lem] >-
-metis_tac [partition_ok_lem] >-
-metis_tac [partition_ok_lem] >-
-metis_tac [partition_ok_lem] >-
+metis_tac [partition_heap_ordered_lem] >-
+metis_tac [partition_heap_ordered_lem] >-
+metis_tac [partition_heap_ordered_lem] >-
+metis_tac [partition_heap_ordered_lem] >-
+metis_tac [partition_heap_ordered_lem] >-
+metis_tac [partition_heap_ordered_lem] >-
 (fs [BAG_EVERY] >>
  metis_tac [transitive_def, WeakLinearOrder, WeakOrder]));
 
-val insert_def = Define `
-insert get_key leq x t =
-  let (a, b) = partition get_key leq x t in
-    Node a x b`;
-
-val merge_def = tDefine "merge" `
-(merge get_key leq Empty h2 = h2) ∧
-(merge get_key leq (Node a x b) h2 =
-  let (ta, tb) = partition get_key leq x h2 in
-    Node (merge get_key leq ta a) x (merge get_key leq tb b))`
-(WF_REL_TAC `measure (\(_,x,y,z).
-                        heap_size (\_.1) y +
-                        heap_size (\_.1) z)` >>
- rw [] >>
- imp_res_tac partition_size >>
- pop_assum (MP_TAC o Q.SPEC `(λ_.1)`) >>
- pop_assum (MP_TAC o Q.SPEC `(λ_.1)`) >>
- full_simp_tac (srw_ss() ++ ARITH_ss) [partition_size]);
-
-val merge_ind = fetch "-" "merge_ind"
-
-val find_min_def = Define `
-(find_min (Node Empty x b) = x) ∧
-(find_min (Node a x b) = find_min a)`;
-
-val find_min_ind = fetch "-" "find_min_ind"
-
-val delete_min_def = Define `
-(delete_min (Node Empty x b) = b) ∧
-(delete_min (Node (Node Empty x b) y c) = Node b y c) ∧
-(delete_min (Node (Node a x b) y c) = Node (delete_min a) x (Node b y c))`;
-
-val delete_min_ind = fetch "-" "delete_min_ind"
-
-val splay_heap_insert_bag = Q.store_thm ("splay_heap_insert_bag",
+val insert_bag = Q.store_thm ("insert_bag",
 `!h get_key leq x.
-  splay_heap_to_bag (insert get_key leq x h) =
-  BAG_INSERT x (splay_heap_to_bag h)`,
+  heap_to_bag (insert get_key leq x h) =
+  BAG_INSERT x (heap_to_bag h)`,
 induct_on `h` >>
-rw [splay_heap_to_bag_def, insert_def] >>
-rw [splay_heap_to_bag_def] >>
+rw [heap_to_bag_def, insert_def] >>
+rw [heap_to_bag_def] >>
 fs [insert_def] >>
 imp_res_tac (GSYM partition_bags) >>
-fs [splay_heap_to_bag_def]);
+fs [heap_to_bag_def]);
 
-val splay_heap_insert_ok = Q.store_thm ("splay_heap_insert_ok",
+val insert_heap_ordered = Q.store_thm ("insert_heap_ordered",
 `!get_key leq x h.
-  WeakLinearOrder leq ∧ splay_heap_ok get_key leq h
+  WeakLinearOrder leq ∧ is_heap_ordered get_key leq h
   ⇒
-  splay_heap_ok get_key leq (insert get_key leq x h)`,
-rw [insert_def, splay_heap_ok_def] >>
-rw [splay_heap_ok_def] >-
-metis_tac [partition_ok] >-
-metis_tac [partition_ok] >-
+  is_heap_ordered get_key leq (insert get_key leq x h)`,
+rw [insert_def, is_heap_ordered_def] >>
+rw [is_heap_ordered_def] >-
+metis_tac [partition_heap_ordered] >-
+metis_tac [partition_heap_ordered] >-
 metis_tac [WeakLinearOrder, WeakOrder, partition_split] >-
-(`BAG_EVERY (\y. ¬leq (get_key y) (get_key x)) (splay_heap_to_bag b)`
+(`BAG_EVERY (\y. ¬leq (get_key y) (get_key x)) (heap_to_bag b)`
            by metis_tac [partition_split, WeakLinearOrder, WeakOrder] >>
  fs [BAG_EVERY] >>
  metis_tac [WeakLinearOrder_neg]));
 
-val splay_heap_merge_bag = Q.store_thm ("splay_heap_merge_bag",
+val merge_bag = Q.store_thm ("merge_bag",
 `!get_key leq h1 h2.
-  (splay_heap_to_bag (merge get_key leq h1 h2) =
-    BAG_UNION (splay_heap_to_bag h1) (splay_heap_to_bag h2))`,
+  (heap_to_bag (merge get_key leq h1 h2) =
+    BAG_UNION (heap_to_bag h1) (heap_to_bag h2))`,
 recInduct merge_ind >>
-rw [merge_def, splay_heap_to_bag_def] >>
+rw [merge_def, heap_to_bag_def] >>
 cases_on `partition get_key leq x h2` >>
 fs [] >>
 imp_res_tac (GSYM partition_bags) >>
-rw [splay_heap_to_bag_def, BAG_UNION_INSERT] >>
+rw [heap_to_bag_def, BAG_UNION_INSERT] >>
 metis_tac [ASSOC_BAG_UNION, COMM_BAG_UNION, BAG_INSERT_commutes]);
 
-val splay_heap_merge_ok = Q.store_thm ("splay_heap_merge_ok",
+val merge_heap_ordered = Q.store_thm ("merge_heap_ordered",
 `!get_key leq h1 h2.
-  WeakLinearOrder leq ∧ splay_heap_ok get_key leq h1 ∧ splay_heap_ok get_key leq h2
+  WeakLinearOrder leq ∧ is_heap_ordered get_key leq h1 ∧ is_heap_ordered get_key leq h2
   ⇒
-  splay_heap_ok get_key leq (merge get_key leq h1 h2)`,
+  is_heap_ordered get_key leq (merge get_key leq h1 h2)`,
 recInduct merge_ind >>
-rw [merge_def, splay_heap_ok_def] >>
-rw [splay_heap_ok_def, splay_heap_merge_bag] >-
-metis_tac [partition_ok] >-
-metis_tac [partition_ok] >-
+rw [merge_def, is_heap_ordered_def] >>
+rw [is_heap_ordered_def, merge_bag] >-
+metis_tac [partition_heap_ordered] >-
+metis_tac [partition_heap_ordered] >-
 metis_tac [partition_split, WeakLinearOrder, WeakOrder] >-
-(`BAG_EVERY (\y. ¬leq (get_key y) (get_key x)) (splay_heap_to_bag tb)`
+(`BAG_EVERY (\y. ¬leq (get_key y) (get_key x)) (heap_to_bag tb)`
            by metis_tac [partition_split, WeakLinearOrder, WeakOrder] >>
  fs [BAG_EVERY] >>
  metis_tac [WeakLinearOrder_neg]));
 
-val splay_heap_find_min_thm = Q.store_thm ("splay_heap_find_min_thm",
+val find_min_correct = Q.store_thm ("find_min_correct",
 `!h get_key leq. 
-  WeakLinearOrder leq ∧ (h ≠ Empty) ∧ splay_heap_ok get_key leq h 
+  WeakLinearOrder leq ∧ (h ≠ Empty) ∧ is_heap_ordered get_key leq h 
   ⇒
-  BAG_IN (find_min h) (splay_heap_to_bag h) ∧
-  (!y. BAG_IN y (splay_heap_to_bag h) ⇒ 
+  BAG_IN (find_min h) (heap_to_bag h) ∧
+  (!y. BAG_IN y (heap_to_bag h) ⇒ 
        leq (get_key (find_min h)) (get_key y))`,
 recInduct find_min_ind >>
-rw [splay_heap_to_bag_def, find_min_def] >>
-fs [splay_heap_ok_def, splay_heap_to_bag_def, BAG_EVERY] >> 
+rw [heap_to_bag_def, find_min_def] >>
+fs [is_heap_ordered_def, heap_to_bag_def, BAG_EVERY] >> 
 metis_tac [WeakLinearOrder, WeakOrder, transitive_def, reflexive_def]);
 
-val splay_heap_delete_min_thm = Q.store_thm ("splay_heap_delete_min_thm",
+val delete_min_correct = Q.store_thm ("delete_min_correct",
 `!h get_key leq.
   WeakLinearOrder leq ∧
   (h ≠ Empty) ∧
-  splay_heap_ok get_key leq h
+  is_heap_ordered get_key leq h
   ⇒
-  splay_heap_ok get_key leq (delete_min h) ∧
-  (splay_heap_to_bag (delete_min h) =
-   BAG_DIFF (splay_heap_to_bag h) (EL_BAG (find_min h)))`,
+  is_heap_ordered get_key leq (delete_min h) ∧
+  (heap_to_bag (delete_min h) =
+   BAG_DIFF (heap_to_bag h) (EL_BAG (find_min h)))`,
 HO_MATCH_MP_TAC delete_min_ind >>
 srw_tac [bagLib.BAG_ss]
-        [delete_min_def, splay_heap_ok_def, splay_heap_to_bag_def,
+        [delete_min_def, is_heap_ordered_def, heap_to_bag_def,
          find_min_def, BAG_INSERT_UNION] >|
 [res_tac >>
      rw [] >>
@@ -284,22 +282,14 @@ srw_tac [bagLib.BAG_ss]
      metis_tac [WeakLinearOrder, WeakOrder, transitive_def],
  res_tac >>
      srw_tac [BAG_AC_ss] [] >>
-     `splay_heap_ok get_key leq (Node v6 v7 v8)` by rw [splay_heap_ok_def] >>
-     `BAG_IN (find_min (Node v6 v7 v8)) (splay_heap_to_bag (Node v6 v7 v8))`
-          by metis_tac [splay_heap_find_min_thm, fetch "-" "heap_distinct"] >>
-     fs [splay_heap_to_bag_def] >>
-     `SUB_BAG (EL_BAG (find_min (Node v6 v7 v8)))
-              (EL_BAG v7 ⊎ (splay_heap_to_bag v6 ⊎ splay_heap_to_bag v8))`
+     `is_heap_ordered get_key leq (Tree v6 v7 v8)` by rw [is_heap_ordered_def] >>
+     `BAG_IN (find_min (Tree v6 v7 v8)) (heap_to_bag (Tree v6 v7 v8))`
+          by metis_tac [find_min_correct, fetch "-" "heap_distinct"] >>
+     fs [heap_to_bag_def] >>
+     `SUB_BAG (EL_BAG (find_min (Tree v6 v7 v8)))
+              (EL_BAG v7 ⊎ (heap_to_bag v6 ⊎ heap_to_bag v8))`
                 by rw [SUB_BAG_EL_BAG] >>
      rw [BAG_UNION_DIFF, SUB_BAG_UNION] >>
      srw_tac [BAG_AC_ss] []]);
 
-val res = translate is_empty_def;
-val res = translate partition_def;
-val res = translate insert_def;
-val res = translate merge_def;
-val res = translate find_min_def;
-val res = translate delete_min_def;
-
 val _ = export_theory()
-
